% Equation 1
\noindent[name= `1']
\begin{dmath}
{C}_{t}^{\left(-{\sigma}\right)}=\frac{{\beta}\, \left(1+{i}_{t}\right)\, {C}_{t+1}^{\left(-{\sigma}\right)}}{{\pi}_{t+1}}
\end{dmath}
% Equation 2
\noindent[name= `2']
\begin{dmath}
\frac{{\gamma}\, {m}_{t}^{\left(-{b}\right)}}{{C}_{t}^{\left(-{\sigma}\right)}}=\frac{{i}_{t}}{1+{i}_{t}}
\end{dmath}
% Equation 3
\noindent[name= `3']
\begin{dmath}
\frac{{\chi}\, {N}_{t}^{{\eta}}}{{C}_{t}^{\left(-{\sigma}\right)}}={w}_{t}
\end{dmath}
% Equation 4
\noindent[name= `phi']
\begin{dmath}
{\varphi}_{t}=\frac{{w}_{t}}{{z}_{t}}
\end{dmath}
% Equation 5
\noindent[name= `Delta']
\begin{dmath}
{\Delta}_{t}=\left(1-{\omega}\right)\, {s}_{t}^{\left(-{\theta}\right)}+{\omega}\, {\pi}_{t}^{{\theta}}\, {\Delta}_{t-1}
\end{dmath}
% Equation 6
\noindent[name= `c']
\begin{dmath}
{C}_{t}=\frac{{N}_{t}\, {z}_{t}}{{\Delta}_{t}}
\end{dmath}
% Equation 7
\noindent[name= `s']
\begin{dmath}
{s}_{t}=\frac{{\theta}\, {g1}_{t}}{\left({\theta}-1\right)\, {g2}_{t}}
\end{dmath}
% Equation 8
\noindent[name= `8']
\begin{dmath}
1=\left(1-{\omega}\right)\, {s}_{t}^{1-{\theta}}+{\omega}\, {\pi}_{t}^{{\theta}-1}
\end{dmath}
% Equation 9
\noindent[name= `g1']
\begin{dmath}
{g1}_{t}={\varphi}_{t}\, {C}_{t}^{1-{\sigma}}+{\beta}\, {\omega}\, {\pi}_{t+1}^{{\theta}}\, {g1}_{t+1}
\end{dmath}
% Equation 10
\noindent[name= `g2']
\begin{dmath}
{g2}_{t}={C}_{t}^{1-{\sigma}}+{\beta}\, {\omega}\, {\pi}_{t+1}^{{\theta}-1}\, {g2}_{t+1}
\end{dmath}
% Equation 11
\noindent[name= `m\_dot']
\begin{dmath}
{\dot{M}}_{t}=\frac{{m}_{t}\, {\pi}_{t}}{{m}_{t-1}}
\end{dmath}
% Equation 12
\noindent[name= `12']
\begin{dmath}
\log\left({\dot{M}}_{t}\right)={\rho_{m}}\, \log\left({\dot{M}}_{t-1}\right)+{\nu}_{t}
\end{dmath}
% Equation 13
\noindent[name= `13']
\begin{dmath}
\log\left({z}_{t}\right)={\rho_z}\, \log\left({z}_{t-1}\right)+{\varepsilon^{z}}_{t}
\end{dmath}
